initial attempts at measures relation

architecture/coq/architecture.v
@@ -1,20 +1,289 @@
-Require Import APDT.
+Require Import ApdtProps.
 
-Module Architecture.
-  
+Module Arch <: APDTMod.
   (** Place identifiers *)
 
-  Inductive Places :=
+  Inductive P :=
   | seL4AM
   | platformAM
   | userAM
   | mpAM.
 
-  Inductive Measures : Places -> Places -> Prop :=
-  | sel4Plat: Measures seL4AM platformAM.
+  Inductive Order: Type :=
+  | SEQ: Order
+  | PAR: Order.
 
+  Inductive APDT: Type :=
+  | USM: APDT
+  | KIM: P -> APDT
+  | SIG: APDT
+  | AT: P -> APDT -> APDT
+  | LN: APDT -> APDT -> APDT
+  | BR: Order -> APDT -> APDT -> APDT.
+
+  Lemma eq_apdt_dec:
+    forall x y: APDT, {x = y} + {x <> y}.
+  Proof.
+  intros.
+  decide equality; decide equality.
+  Defined.
+  Hint Resolve eq_apdt_dec.
+
+(** The example *)
+
+Definition ex :=
+  AT seL4AM (LN (BR PAR (KIM platformAM)
+                   (AT platformAM (LN USM SIG))) SIG).
+
+(** Another example *)
+
+Definition aex :=
+  AT seL4AM (LN (LN (KIM platformAM)
+                    (AT platformAM (LN USM SIG))) SIG).
+
+(** Evidence Forms *)
+
+Inductive Ev: Type :=
+| Mt: Ev                     (* Empty evidence *)
+| N: P -> Ev                  (* Nonce evidence *)
+| K: P -> P -> Ev              (* Kernel measurement *)
+| U: P -> Ev                  (* User space measurement *)
+| G: Ev -> P -> Ev             (* Signature *)
+| SS: Ev -> Ev -> Ev           (* Really should be S, but conflicts *)
+| PP: Ev -> Ev -> Ev.           (* Parallel *)
+
+Theorem eq_ev_dec :
+  forall x y: Ev, {x = y} + {x <> y}.
+Proof.
+  intros.
+  decide equality; decide equality.
+Defined.
+Hint Resolve eq_ev_dec.
+
+Inductive is_Mt : Ev -> Prop :=
+| isMt : is_Mt Mt.
+Hint Constructors is_Mt.
+
+Definition is_Mt_dec : forall e, {is_Mt e} + {~ is_Mt e}.
+Proof.
+  intros.
+  destruct e; try (right; unfold not; intros; inversion H; contradiction).
+  left. eauto.
+Defined.
+
+(** * Denotational Semantics
+
+    The evidence associated with a APDT *)
+
+Definition sequ e1 e2: Ev :=
+  match e1 with
+  | Mt => e2
+  | _ => SS e1 e2
+  end.
+
+Definition para e1 e2: Ev :=
+  match (e1, e2) with
+  | (Mt, _) => e2
+  | (_, Mt) => e1
+  | _ => PP e1 e2
+  end.
+
+Fixpoint eval (t: APDT) (p: P) (e: Ev): Ev :=
+  match t with
+  | KIM q => sequ e (K q p)
+  | USM => sequ e (U p)
+  | SIG => G e p
+  | AT q t => eval t q e
+  | LN t1 t2 =>
+    eval t2 p (eval t1 p e)
+  | BR SEQ t1 t2 =>
+    sequ (eval t1 p e) (eval t2 p e)
+  | BR PAR t1 t2 =>
+    para (eval t1 p e) (eval t2 p e)
+  end.
+
+(** * Properties *)
+
+(** Equivalent APDTs *)
+
+Definition equiv_terms t1 t2 :=
+  forall e p, eval t1 p e = eval t2 p e.
+
+Lemma at_at:
+  forall p q t,
+    equiv_terms (AT p (AT q t)) (AT q t).
+Proof.
+  unfold equiv_terms.
+  intros; simpl; auto.
+Qed.
+
+(** Facts about [sequ] and [para] *)
+
+Ltac inv H := inversion H; clear H; subst.
+
+Lemma sequ_mt:
+  forall e f,
+    sequ e f = Mt -> e = Mt /\ f = Mt.
+Proof.
+  intros e f H; destruct e; destruct f;
+    auto; simpl in H; inv H.
+Qed.
+
+Lemma para_mt:
+  forall e f,
+    para e f = Mt -> e = Mt /\ f = Mt.
+Proof.
+  intros e f H; destruct e; destruct f;
+    auto; simpl in H; inv H.
+Qed.
+
+Lemma sequ_mt_e:
+  forall e,
+    sequ Mt e = e.
+Proof.
+  intros; simpl; auto.
+Qed.
+
+Lemma sequ_SS:
+  forall e f,
+    e <> Mt -> sequ e f = SS e f.
+Proof.
+  intros; destruct e; simpl; auto; tauto.
+Qed.
+
+Lemma para_mt_e:
+  forall e,
+    para Mt e = e.
+Proof.
+  intros; simpl; auto.
+Qed.
+
+Lemma para_e_mt:
+  forall e,
+    para e Mt = e.
+Proof.
+  intros; destruct e; simpl; auto.
+Qed.
+
+Lemma para_P:
+  forall e f,
+    e <> Mt -> f <> Mt -> para e f = PP e f.
+Proof.
+  intros; destruct e; destruct f; simpl; auto; tauto.
+Qed.
+
+(** No term is associated with the empty evidence form. *)
+
+Lemma eval_not_mt:
+  forall e p t,
+    eval t p e <> Mt.
+Proof. 
+  intros e p t.
+  revert p.
+  revert e.
+  induction t; intros; intro; simpl in H; auto.
+  - destruct e; auto; inv H.
+  - destruct e; auto; inv H.
+  - destruct e; auto; inv H.
+  - apply IHt in H; auto.
+  - apply IHt2 in H; auto.
+  - destruct o.
+    + destruct (eval t1 p e);
+        try (simpl in H; congruence).
+    + apply para_mt in H. destruct H. apply IHt1 in H. inversion H.
+Qed.
+Hint Resolve eval_not_mt.
+
+Lemma sequ_eval_SS:
+  forall e1 e2 p1 t1,
+    sequ (eval t1 p1 e1) e2 =
+    SS (eval t1 p1 e1) e2.
+Proof.
+  intros; apply sequ_SS; apply eval_not_mt.
+Qed.
+
+Lemma para_eval_P:
+  forall e1 e2 p1 p2 t1 t2,
+    para (eval t1 p1 e1) (eval t2 p2 e2) =
+    PP (eval t1 p1 e1) (eval t2 p2 e2).
+Proof.
+  intros; apply para_P; apply eval_not_mt.
+Qed.
+
+(** [eval] is injective on evidence forms. *)
+
+Lemma eval_inj:
+  forall e f p t,
+    eval t p e = eval t p f -> e = f.
+Proof.
+  intros.
+  revert H.
+  revert p.
+  revert f.
+  revert e.
+  induction t; intros; simpl in H.
+  - destruct e; destruct f; inv H; auto.
+  - destruct e; destruct f; inv H; auto.
+  - destruct e; destruct f; inv H; auto.
+  - apply IHt in H; auto.
+  - eauto.
+  - destruct o.
+    + simpl in H;
+        rewrite sequ_eval_SS in H;
+        rewrite sequ_eval_SS in H;
+        inv H.
+    eauto.
+    + simpl in H;
+        rewrite para_eval_P in H;
+        rewrite para_eval_P in H;
+        inv H.
+    eauto.
+Qed.
   
+Inductive Measures : APDT -> P -> P -> Prop :=
+| dirKIM: forall a, forall p1 p2, a=(AT p1 (KIM p2)) -> Measures a p1 p2
+| seqKIMl: forall a b c, forall p1 p2, a=(AT p1 (LN b c)) -> Measures b p1 p2 -> Measures a p1 p2
+| seqKIMr: forall a b c, forall p1 p2, a=(AT p1 (LN b c)) -> Measures c p1 p2 -> Measures a p1 p2
+| parKIMl: forall a b c, forall d, forall p1 p2, a=(AT p1 (BR d b c)) -> Measures b p1 p2 -> Measures a p1 p2
+| parKIMr: forall a b c, forall d, forall p1 p2, a=(AT p1 (BR d b c)) -> Measures c p1 p2 -> Measures a p1 p2.
+
+Hint Constructors Measures.
+
+Definition ex1 := (AT seL4AM (KIM platformAM)).
+
+Lemma ex1l: Measures ex1 seL4AM platformAM.
+Proof.
+  auto.
+Qed.
+
+Definition ex2 := (AT seL4AM (LN (USM) (KIM platformAM))).
+
+Lemma ed2l: Measures ex1 seL4AM platformAM.
+Proof.
+  auto.
+Qed.
   
-  
-End Architecture.
-       
+Definition ex3 := (AT seL4AM (LN (KIM platformAM) (USM))).
+
+Lemma ed3l: Measures ex1 seL4AM platformAM.
+Proof.
+  auto.
+Qed.
+
+Definition ex4 := (AT seL4AM (BR PAR (KIM platformAM) (USM))).
+
+Lemma ed4l: Measures ex1 seL4AM platformAM.
+Proof.
+  auto.
+Qed.
+
+Definition ex5 := (AT seL4AM (BR SEQ (KIM platformAM) (USM))).
+
+Lemma ed5l: Measures ex1 seL4AM platformAM.
+Proof.
+  auto.
+Qed.
+
+Definition ex :=
+  AT seL4AM (LN (BR PAR (KIM platformAM)
+                   (AT platformAM (LN USM SIG))) SIG).
